* AADL Thread as DEVS component: implement periodic dispatch

src/AADL/behavior/thread.v
@@ -29,9 +29,12 @@
  *
  * DM21-0762
 ***)
-(** %\chapter{AADL Threads} %*)
+(*|
+AADL Threads
+============
+|*)
 
-(* begin hide *)
+(*| .. coq:: none |*)
 (** Coq Library *)
 Require Import List.
 Import ListNotations. (* from List *)
@@ -47,6 +50,7 @@ Import IfNotations.
 Require Import Oqarina.coq_utils.all.
 
 Require Import Oqarina.core.all.
+Import NaturalTime.
 Require Import Oqarina.AADL.Kernel.all.
 Require Import Oqarina.AADL.property_sets.all.
 
@@ -54,60 +58,87 @@ Require Import Oqarina.AADL.declarative.all.
 Require Import Oqarina.AADL.instance.all.
 Require Import Oqarina.AADL.behavior.port_variable.
 
-Open Scope Z_scope.
-(* end hide *)
+Require Import Oqarina.formalisms.DEVS.parallel.all.
+Require Import Oqarina.formalisms.all.
 
-(** * Thread State Variable *)
+Import AADL_Notations.
+Open Scope aadl_scope.
 
-(** %\N% Each AADL thread is associated to a state variable that stores the relevant parameters relative to is dispatch and scheduling by the underlying executive. *)
+Open Scope nat_scope.
 
-(* begin hide*)
+(*| .. coq:: |*)
+
+(*|
+
+Thread State Variable
+---------------------
+
+Each AADL thread is associated to a state variable that stores the relevant parameters relative to is dispatch and scheduling by the underlying executive.
+|*)
+
+(*| .. coq:: none |*)
 Section Thread_State_Variable.
-(* end hide *)
+(*| .. coq:: |*)
 
-(** [Build_Dispatch_Trigger] returns the list of triggering features *)
+(*| :coq:`Build_Dispatch_Trigger` returns the list of triggering features |*)
 
-  Definition Build_Dispatch_Trigger (l : list feature) :=
-    filter Is_Triggering_Feature l. (* %\change{should use also property Dispatch\_Trigger}% *)
+Definition Build_Dispatch_Trigger (l : list feature) :=
+  filter Is_Triggering_Feature l.
+  (* XXX should use also property Dispatch\_Trigger *)
 
-(** %\begin{definition}[Thread State (Coq)]
-TBD
-  \end{definition} %*)
-  Inductive thread_state := Idle | Ready | Running.
+Inductive thread_state := Not_Activated | Idle | Ready | Running.
 
-  Record thread_state_variable : Type := {
-    (* static configuration parameters derived from AADL thread component *)
-    dispatch_protocol : Dispatch_Protocol;
-    period : AADL_Time;
-    deadline : AADL_Time;
-    priority : Z;
-    dispatch_able : bool;
-    (* wcet : AADL_Time; *)
+(*| :coq:`thread_state_variable` defines the general state variable that stores
+the current state of a thread. Its is made of a static part that is derived
+from the AADL model, and a dynamic part that is the current state used in the simulation. It is associated with a constructor :coq:`mk_thread_state_variable` and a well-formedness predicate. |*)
 
-    (* dynamic status *)
-    clock : AADL_Time;                      (* current clock *)
-    current_state : thread_state;
-    dispatch_time : AADL_Time;
-    input_ports : list port_variable;
-    output_ports : list port_variable;
-    dispatch_trigger : list feature;
-  }.
+Record thread_state_variable : Type := {
+  (* static configuration parameters derived from AADL thread component *)
+  dispatch_protocol : Dispatch_Protocol;
+  period : Time;
+  deadline : AADL_Time;
+  priority : Z;
+  dispatch_able : bool;
+  wcet : Time;
 
-  Definition mk_thread_state_variable (t : component) : thread_state_variable := {|
-    dispatch_protocol := Map_Dispatch_Protocol (t->properties);
-    period := Map_Period (t->properties);
-    priority := Map_Priority (t->properties);
-    deadline := Map_Deadline (t->properties);
-    dispatch_able := Map_Dispatch_Able (t->properties);
+  (* dynamic status *)
+  clock : Time; (* clock with reset for evaluating dispatch *)
+  cet : Time;   (* execution time clock *)
+  delta_cet : Time ;
+  current_state : thread_state;
+  next_dispatch_time : Time;
+  input_ports : list port_variable;
+  output_ports : list port_variable;
+  dispatch_trigger : list feature;
+}.
 
-    clock := 0;
-    dispatch_time := 0;
-    current_state := Idle;
-    input_ports := Build_Input_Port_Variables (t->features);
-    output_ports := Build_Output_Port_Variables (t->features);
-    dispatch_trigger := Build_Dispatch_Trigger (t->features);
-  |}.
+(*| * :coq:`mk_thread_state_variable` maps an AADL component to a :coq:`thread_state_variable`.|*)
+Definition mk_thread_state_variable (t : component) : thread_state_variable := {|
+  dispatch_protocol := Map_Dispatch_Protocol (t->properties);
+  period := (Z.to_nat (Map_Period (t->properties))) ;
+  priority := Map_Priority (t->properties);
+  deadline := Map_Deadline (t->properties);
+  dispatch_able := Map_Dispatch_Able (t->properties);
+  wcet := Z.to_nat (snd (Map_Compute_Execution_Time (t->properties)));
 
+  clock := Zero;
+  cet := Zero;
+  delta_cet := Zero;
+  next_dispatch_time := Zero;
+  current_state := Not_Activated;
+  input_ports := Build_Input_Port_Variables (t->features);
+  output_ports := Build_Output_Port_Variables (t->features);
+  dispatch_trigger := Build_Dispatch_Trigger (t->features);
+|}.
+
+(*| :coq:`Compute_Entrypoint` defines the compute entrypoint of a thread. |*)
+
+Definition Compute_Entry_Point := thread_state_variable -> thread_state_variable.
+
+Definition Default_Compute_Entry_Point : Compute_Entry_Point :=
+  (fun x => x).
+
+(*| .. coq:: none |*)
   Definition thread_state_variable_wf (t : thread_state_variable) :=
     t.(dispatch_protocol) <> Unspecified_Dispatch_Protocol /\
     port_variable_list_wf t.(input_ports) /\
@@ -126,10 +157,10 @@ TBD
     - apply port_variable_list_wf_dec.
     - apply port_variable_list_wf_dec.
   Qed.
+(*| .. coq:: |*)
 
-(* begin hide *)
+(*| .. coq:: none |*)
 End Thread_State_Variable.
-(* end hide*)
 
 Ltac prove_thread_state_variable_wf :=
   repeat match goal with
@@ -140,246 +171,265 @@ Ltac prove_thread_state_variable_wf :=
     | |- NoDup  _  => apply NoDup_cons ; auto
     | |- NoDup nil => apply NoDup_nil
   end.
+(*| .. coq:: |*)
 
-(** * Thread Dispatching
+(*|
 
-%\N% This section captures the content of %\S 5.4.2 of \cite{as2-cArchitectureAnalysisDesign2017}%. Ultimately, we want to provide a definition of the [Enabled] function that controls the dispatch of a thread. The definition of this function relies on the state of some of its triggering features. In the following, we use directly the concept of thread state variable and port variables to define the [Enabled] function. *)
+Thread Dispatching
+------------------
 
-(* begin hide *)
+This section captures the content of %\S 5.4.2 of \cite{as2-cArchitectureAnalysisDesign2017}%. Ultimately, we want to provide a definition of the :coq:`Enabled` function that controls the dispatch of a thread. The definition of this function relies on the state of some of its triggering features. In the following, we use directly the concept of thread state variable and port variables to define :coq:`Enabled` .
+
+|*)
+
+(*| .. coq:: none |*)
 Section AADL_Dispatching.
-(* end hide *)
+(*| .. coq::  |*)
 
-(** ** Intermediate Predicates
+(*|
 
-%\N% All AADL dispatch protocols review the state of triggering features and the current clock. We build the [Thread_Has_Activated_Triggering_Feature] predicate as a conjunction of more basic predicates, in [Prop], and demonstrate their decidability.
+Intermediate Predicates
+^^^^^^^^^^^^^^^^^^^^^^^
 
-%\N% First, we check whether the feature is activated, [Is_Feature_Activated], then whether it is in the dispatch trigger, in [Feature_In_Dispatch_Trigger]. *)
+All AADL dispatch protocols review the state of triggering features and the current clock. We build the :coq:`Thread_Has_Activated_Triggering_Feature` predicate as a conjunction of more basic predicates, in :coq:`Prop`, and demonstrate their decidability.
 
-  Definition Is_Feature_Activated (p : port_variable) :=
-    ~ PortQueue.Is_Empty p.(outer_variable).
+First, we check whether the feature is activated, :coq:`Is_Feature_Activated`, then whether it is in the dispatch trigger, in :coq:`Feature_In_Dispatch_Trigger`.
 
-  (* begin hide *)
-  Lemma Is_Feature_Activated_dec :
-    forall (p : port_variable), dec_sumbool (Is_Feature_Activated p).
-  Proof.
-    prove_dec.
-    apply PortQueue.Is_Empty_dec.
-  Defined.
-  (* end hide *)
+|*)
 
-  Definition Feature_In_Dispatch_Trigger (p : port_variable) (d : list feature) :=
-    In p.(port) d.
+Definition Is_Feature_Activated (p : port_variable) :=
+  ~ PortQueue.Is_Empty p.(outer_variable).
 
-  (* begin hide *)
-  Definition Feature_In_Dispatch_Trigger_dec :
-    forall (p : port_variable) (d : list feature),
-      dec_sumbool (Feature_In_Dispatch_Trigger p d).
-  Proof.
-    prove_dec2.
-    apply feature_eq_dec.
-  Defined.
-  (* end hide *)
+(*| .. coq:: none |*)
+Lemma Is_Feature_Activated_dec :
+  forall (p : port_variable), dec_sumbool (Is_Feature_Activated p).
+Proof.
+  prove_dec.
+  apply PortQueue.Is_Empty_dec.
+Defined.
+(*| .. coq::  |*)
 
-  (** %\N% From that point, we can build [Thread_Has_Activated_Triggering_Feature] that is true iff. the thread has at least one activated triggering feature that is also in the dispatch trigger. *)
+Definition Feature_In_Dispatch_Trigger (p : port_variable) (d : list feature) :=
+  In p.(port) d.
 
-  Definition Is_Activated_Triggering_Feature (p : port_variable)  (d : list feature) :=
-    Is_Feature_Activated p /\ Feature_In_Dispatch_Trigger p d.
+(*| .. coq:: none |*)
+Definition Feature_In_Dispatch_Trigger_dec :
+  forall (p : port_variable) (d : list feature),
+    dec_sumbool (Feature_In_Dispatch_Trigger p d).
+Proof.
+  prove_dec2.
+Defined.
+(*| .. coq::  |*)
 
-  (* begin hide *)
-  Lemma Is_Activated_Triggering_Feature_dec:
-    forall (p : port_variable)  (d : list feature),
-      dec_sumbool (Is_Activated_Triggering_Feature p d).
-  Proof.
-    prove_dec2.
-    apply Is_Feature_Activated_dec.
-    apply feature_eq_dec.
-  Defined.
-  (* end hide *)
+(*| From that point, we can build :coq:`Thread_Has_Activated_Triggering_Feature` that is true iff. the thread has at least one activated triggering feature that is also in the dispatch trigger.
+|*)
 
-  Definition Is_Activated_Triggering_Feature_b (p : port_variable)  (d : list feature) :=
-    if Is_Activated_Triggering_Feature_dec p d is (left _) then true else false.
+Definition Is_Activated_Triggering_Feature (p : port_variable)  (d : list feature) :=
+  Is_Feature_Activated p /\ Feature_In_Dispatch_Trigger p d.
 
-  Definition Has_Activated_Triggering_Feature (l : list port_variable) (d : list feature) :=
-    All_Or (fun x => (Is_Activated_Triggering_Feature x d)) l.
+(*| .. coq:: none |*)
+Lemma Is_Activated_Triggering_Feature_dec:
+  forall (p : port_variable)  (d : list feature),
+    dec_sumbool (Is_Activated_Triggering_Feature p d).
+Proof.
+  prove_dec2.
+  apply Is_Feature_Activated_dec.
+Defined.
 
-  (* begin hide *)
-  Lemma Has_Activated_Triggering_Feature_dec :
-    forall (l : list port_variable) (d : list feature),
-      dec_sumbool (Has_Activated_Triggering_Feature l d).
-  Proof.
-    intros.
-    unfold dec_sumbool.
-    unfold Has_Activated_Triggering_Feature.
-    induction l.
-    - auto.
-    - unfold All_Or. apply dec_sumbool_or.
-      * apply Is_Activated_Triggering_Feature_dec.
-      * apply IHl.
-  Defined.
-  (* end hide *)
+Definition Is_Activated_Triggering_Feature_b (p : port_variable)  (d : list feature) :=
+  if Is_Activated_Triggering_Feature_dec p d is (left _) then true else false.
+(*| .. coq::  |*)
 
-  Definition Thread_Has_Activated_Triggering_Feature (th : thread_state_variable) :=
-    Has_Activated_Triggering_Feature
-      th.(input_ports) th.(dispatch_trigger).
+Definition Has_Activated_Triggering_Feature
+  (l : list port_variable) (d : list feature)
+:=
+  All_Or (fun x => (Is_Activated_Triggering_Feature x d)) l.
 
-  (* begin hide *)
+(*| .. coq:: none |*)
+Lemma Has_Activated_Triggering_Feature_dec :
+  forall (l : list port_variable) (d : list feature),
+    { Has_Activated_Triggering_Feature l d } + { ~ Has_Activated_Triggering_Feature l d }.
+Proof.
+  intros.
+  unfold Has_Activated_Triggering_Feature.
+  induction l.
+  - auto.
+  - unfold All_Or. apply dec_sumbool_or.
+    * apply Is_Activated_Triggering_Feature_dec.
+    * apply IHl.
+Defined.
+(*| .. coq::  |*)
+
+Definition Thread_Has_Activated_Triggering_Feature
+  (th : thread_state_variable)
+  :=
+  Has_Activated_Triggering_Feature th.(input_ports) th.(dispatch_trigger).
+
+  (*| .. coq:: none |*)
   Lemma Thread_Has_Activated_Triggering_Feature_dec :
     forall (th : thread_state_variable),
-      dec_sumbool (Thread_Has_Activated_Triggering_Feature th).
+      { Thread_Has_Activated_Triggering_Feature th } +
+      { ~ Thread_Has_Activated_Triggering_Feature th }.
   Proof.
-    unfold dec_sumbool.
-    unfold Thread_Has_Activated_Triggering_Feature.
-    unfold Has_Activated_Triggering_Feature.
-    intros.
-    apply Has_Activated_Triggering_Feature_dec.
+    generalize Has_Activated_Triggering_Feature_dec.
+    prove_dec.
   Defined.
-(* end hide *)
+(*| .. coq::  |*)
 
-(** ** Definition of [Enabled]
+(*|
 
-%\N% From the previous definitions, we can now define the [Enabled] function that returns [true] when a thread is dispatched.
+Definition of :coq:`Enabled`
+^^^^^^^^^^^^^^^^^^^^^^^^^^^^
+
+From the previous definitions, we can now define the :coq:`Enabled` function that returns :coq:`true` when a thread is dispatched.
 
 A thread can be enable if it is "dispatchable". Then, we define basic predicates for each dispatch protocol.
-*)
+|*)
 
-  Definition Thread_Dispatchable (th : thread_state_variable) :=
-    (th.(dispatch_able) = true).
+Definition Thread_Dispatchable (th : thread_state_variable) :=
+  (th.(dispatch_able) = true).
 
-  Lemma Thread_Dispatchable_dec:
-    forall (th : thread_state_variable), dec_sumbool (Thread_Dispatchable th).
-  Proof.
-    prove_dec.
-    apply bool_dec.
-  Defined.
+(*| .. coq:: none |*)
+Lemma Thread_Dispatchable_dec:
+  forall (th : thread_state_variable), dec_sumbool (Thread_Dispatchable th).
+Proof.
+  prove_dec.
+  apply bool_dec.
+Defined.
+(*| .. coq:: |*)
 
-  Definition Periodic_Enabled (th : thread_state_variable) :=
-    (Thread_Dispatchable th) /\ (th.(clock) mod th.(period) = 0).
+Definition Periodic_Enabled (th : thread_state_variable) :=
+  (Thread_Dispatchable th) /\ (th.(clock) mod th.(period) = 0).
 
-  (* begin hide *)
-  Lemma Periodic_Enabled_dec:
-    forall (th : thread_state_variable), dec_sumbool (Periodic_Enabled th).
-  Proof.
-    prove_dec.
-    apply Thread_Dispatchable_dec.
-    apply Z.eq_dec.
-  Defined.
-  (* end hide *)
+(*| .. coq:: none |*)
+Lemma Periodic_Enabled_dec:
+  forall (th : thread_state_variable), dec_sumbool (Periodic_Enabled th).
+Proof.
+  prove_dec.
+  apply Thread_Dispatchable_dec.
+  apply PeanoNat.Nat.eq_dec.
+Defined.
+(*| .. coq::  |*)
 
-  Definition Aperiodic_Enabled (th : thread_state_variable) :=
-    (Thread_Dispatchable th) /\
-      (Thread_Has_Activated_Triggering_Feature th).
+Definition Aperiodic_Enabled (th : thread_state_variable) :=
+  (Thread_Dispatchable th) /\
+    (Thread_Has_Activated_Triggering_Feature th).
 
-  (* begin hide *)
-  Lemma Aperiodic_Enabled_dec:
-    forall (th : thread_state_variable), dec_sumbool (Aperiodic_Enabled th).
-  Proof.
-    prove_dec.
-    apply Thread_Dispatchable_dec.
-    apply Thread_Has_Activated_Triggering_Feature_dec.
-  Defined.
-  (* end hide *)
+(*| .. coq:: none |*)
+Lemma Aperiodic_Enabled_dec:
+  forall (th : thread_state_variable), dec_sumbool (Aperiodic_Enabled th).
+Proof.
+  prove_dec.
+  apply bool_dec.
+  apply Thread_Has_Activated_Triggering_Feature_dec.
+Defined.
+(*| .. coq::  |*)
 
-  Definition Sporadic_Enabled (th : thread_state_variable) :=
-    (Thread_Dispatchable th) /\
-      th.(period) <= th.(clock) /\
-      Thread_Has_Activated_Triggering_Feature th.
-
-  (* begin hide *)
-  Lemma Sporadic_Enabled_dec:
-    forall (th : thread_state_variable), dec_sumbool (Sporadic_Enabled th).
-  Proof.
-    prove_dec.
-    apply Thread_Dispatchable_dec.
-    apply Z_le_dec.
-    apply Thread_Has_Activated_Triggering_Feature_dec.
-  Defined.
-  (* end hide *)
-
-  Definition Timed_Enabled (th : thread_state_variable) :=
-    (Thread_Dispatchable th) /\
-    ((th.(period) = th.(clock)) \/
-    Thread_Has_Activated_Triggering_Feature th).
-
-  (* begin hide *)
-  Lemma Timed_Enabled_dec:
-    forall (th : thread_state_variable), dec_sumbool (Timed_Enabled th).
-  Proof.
-    prove_dec.
-    apply Thread_Dispatchable_dec.
-    apply Z.eq_dec.
-    apply Thread_Has_Activated_Triggering_Feature_dec.
-  Defined.
-  (* end hide *)
-
-  Definition Hybrid_Enabled (th : thread_state_variable) :=
-    (Thread_Dispatchable th) /\ (th.(period) = th.(clock)) /\
+Definition Sporadic_Enabled (th : thread_state_variable) :=
+  (Thread_Dispatchable th) /\
+    th.(period) <= th.(clock) /\
     Thread_Has_Activated_Triggering_Feature th.
 
-  (* begin hide *)
-  Lemma Hybrid_Enabled_dec:
-    forall (th : thread_state_variable), dec_sumbool (Hybrid_Enabled th).
-  Proof.
-    prove_dec.
-    apply Thread_Dispatchable_dec.
-    apply Z.eq_dec.
-    apply Thread_Has_Activated_Triggering_Feature_dec.
-  Defined.
-  (* end hide *)
+(*| .. coq:: none |*)
+Lemma Sporadic_Enabled_dec:
+  forall (th : thread_state_variable), dec_sumbool (Sporadic_Enabled th).
+Proof.
+  generalize bool_dec.
+  generalize Thread_Has_Activated_Triggering_Feature_dec.
+  prove_dec.
+  apply Compare_dec.le_dec.
+Defined.
+(*| .. coq::  |*)
 
-  Definition Background_Enabled (th : thread_state_variable) :=
-    (Thread_Dispatchable th).
+Definition Timed_Enabled (th : thread_state_variable) :=
+  (Thread_Dispatchable th) /\
+  ((th.(period) = th.(clock)) \/
+  Thread_Has_Activated_Triggering_Feature th).
 
-  (* begin hide *)
-  Lemma Background_Enabled_dec:
-    forall (th : thread_state_variable), dec_sumbool (Background_Enabled th).
-  Proof.
-    prove_dec.
-    apply Thread_Dispatchable_dec.
-  Defined.
-  (* end hide *)
+(*| .. coq:: none |*)
+Lemma Timed_Enabled_dec:
+  forall (th : thread_state_variable), dec_sumbool (Timed_Enabled th).
+Proof.
+  prove_dec.
+  apply Thread_Dispatchable_dec.
+  apply PeanoNat.Nat.eq_dec.
+  apply Thread_Has_Activated_Triggering_Feature_dec.
+Defined.
+(*| .. coq::  |*)
 
-  (** %\N% Then we define the [Enabled] predicate *)
+Definition Hybrid_Enabled (th : thread_state_variable) :=
+  (Thread_Dispatchable th) /\ (th.(period) = th.(clock)) /\
+  Thread_Has_Activated_Triggering_Feature th.
 
-  Definition Enabled (th : thread_state_variable) :=
-    match th.(dispatch_protocol) with
-    | Periodic => Periodic_Enabled th
-    | Sporadic => Sporadic_Enabled th
-    | Aperiodic => Aperiodic_Enabled th
-    | Timed => Timed_Enabled th
-    | Hybrid => Hybrid_Enabled th
-    | Background => Background_Enabled th
-    | Unspecified => False
-    end.
+(*| .. coq:: none |*)
+Lemma Hybrid_Enabled_dec:
+  forall (th : thread_state_variable), dec_sumbool (Hybrid_Enabled th).
+Proof.
+  prove_dec.
+  apply Thread_Dispatchable_dec.
+  apply PeanoNat.Nat.eq_dec.
+  apply Thread_Has_Activated_Triggering_Feature_dec.
+Defined.
+(*| .. coq::  |*)
 
-  (* begin hide *)
-  Lemma Enabled_dec: forall (th : thread_state_variable), dec_sumbool (Enabled th).
-  Proof.
-    prove_dec.
-    destruct (dispatch_protocol th).
-    auto.
-    apply Periodic_Enabled_dec.
-    apply Sporadic_Enabled_dec.
-    apply Aperiodic_Enabled_dec.
-    apply Background_Enabled_dec.
-    apply Timed_Enabled_dec.
-    apply Hybrid_Enabled_dec.
-  Defined.
-  (* end hide *)
+Definition Background_Enabled (th : thread_state_variable) :=
+  (Thread_Dispatchable th).
 
-  (** [Enabled_oracle] return a [bool] as a witness, for debugging purposes. *)
+(*| .. coq:: none |*)
+Lemma Background_Enabled_dec:
+  forall (th : thread_state_variable), dec_sumbool (Background_Enabled th).
+Proof.
+  prove_dec.
+  apply Thread_Dispatchable_dec.
+Defined.
+(*| .. coq::  |*)
+
+(*| Then we define the :coq:`Enabled` predicate |*)
+
+Definition Enabled (th : thread_state_variable) :=
+  match th.(dispatch_protocol) with
+  | Periodic => Periodic_Enabled th
+  | Sporadic => Sporadic_Enabled th
+  | Aperiodic => Aperiodic_Enabled th
+  | Timed => Timed_Enabled th
+  | Hybrid => Hybrid_Enabled th
+  | Background => Background_Enabled th
+  | Unspecified => False
+  end.
+
+(*| .. coq:: none |*)
+Lemma Enabled_dec: forall (th : thread_state_variable),
+  dec_sumbool (Enabled th).
+Proof.
+  prove_dec.
+  destruct (dispatch_protocol th).
+  auto.
+  apply Periodic_Enabled_dec.
+  apply Sporadic_Enabled_dec.
+  apply Aperiodic_Enabled_dec.
+  apply Background_Enabled_dec.
+  apply Timed_Enabled_dec.
+  apply Hybrid_Enabled_dec.
+Defined.
+(*| .. coq::  |*)
+
+  (** :coq:`Enabled_oracle` return a :coq:`bool` as a witness, for debugging purposes. *)
 
   Definition Enabled_oracle (th : thread_state_variable) :=
     if Enabled_dec th is (left _) then true else false.
 
-(* begin hide *)
+(*| .. coq:: none |*)
 End AADL_Dispatching.
-(* end hide *)
+(*| .. coq::  |*)
 
-(** ** Ports Queue Processing *)
+(*|
 
-(**  %\N% The following is a first cut at formalizing ports from %\S 8.3%. We capture the definition of [Frozen] for ports. First, we build ATF, the list of Activated Triggering Features. *)
+Ports Queue Processing
+----------------------
 
-(** - [Activated_Triggering_Features] returns the list of Activated Triggering Features. *)
+The following is a first cut at formalizing ports from %\S 8.3%. We capture the definition of :coq:`Frozen` for ports. First, we build ATF, the list of Activated Triggering Features. |*)
+
+(*| - :coq:`Activated_Triggering_Features` returns the list of Activated Triggering Features. |*)
 
 Definition Activated_Triggering_Features'  (l : list port_variable) (d : list feature) :=
   filter (fun x => Is_Activated_Triggering_Feature_b x d) l.
@@ -387,37 +437,24 @@ Definition Activated_Triggering_Features'  (l : list port_variable) (d : list fe
 Definition Activated_Triggering_Features (th : thread_state_variable) :=
   Activated_Triggering_Features' th.(input_ports) th.(dispatch_trigger).
 
-(** - [Get_Port_Variable_With_Max_Urgency] returns the port variable with the maximum urgency, see %\S 8.3 (32) \change{We should also address the FIFO for ports with same urgency .. }% *)
-
-Fixpoint Get_Port_Variable_With_Max_Urgency
-  (p : port_variable) (l : list port_variable) : port_variable :=
-    match l with
-    | nil => p
-    | h :: t => if p.(urgency) <=? h.(urgency) then
-        Get_Port_Variable_With_Max_Urgency h t else
-        Get_Port_Variable_With_Max_Urgency p t
-      (* note we take h in all cases, this is to address the case where the
-        first argument is [Invalid_Port_Variable] *)
-    end.
-
-(** %\N% Then, we can define the [Get_Elected_Triggering_Feature] that returns the elected features among Activated Triggering Features. *)
+(*| Then, we can define the :coq:`Get_Elected_Triggering_Feature` that returns the elected features among Activated Triggering Features. |*)
 
 Definition Get_Elected_Triggering_Feature (th : thread_state_variable) : port_variable :=
   Get_Port_Variable_With_Max_Urgency Invalid_Port_Variable
       (Activated_Triggering_Features th).
 
-(** %\N% [Current_Valid_IO_Time_Spec] returns the current IO_Time_Spec for the considered port variable. A port variable can be associated with a list of IO_Time_Spec. The current IO_Time_Spec denotes the IO_Time_Spec that is current to the thread state. %\change{This version is highly simplified. We should define this in the standard first}% *)
+(*| :coq:`Current_Valid_IO_Time_Spec` returns the current IO_Time_Spec for the considered port variable. A port variable can be associated with a list of IO_Time_Spec. The current IO_Time_Spec denotes the IO_Time_Spec that is current to the thread state. %\change{This version is highly simplified. We should define this in the standard first}% |*)
 
 Definition Current_Valid_IO_Time_Spec (p : port_variable) (th : thread_state_variable) :=
   hd Unspecified_IO_Time_Spec (projectionIO_Time_Spec p.(port_input_times)).
 
-(** %\N% The definition of the [Frozen] predicate relies on the previous definitions. A port variable is frozen based on the current thread state, the port IO_Time_Spec, etc.*)
+(*| The definition of the :coq:`Frozen` predicate relies on the previous definitions. A port variable is frozen based on the current thread state, the port IO_Time_Spec, etc. |*)
 
 Definition Dispatch_Frozen (p : port_variable) (th : thread_state_variable) : Prop :=
    (p = Get_Elected_Triggering_Feature  th) \/
        ~ (Feature_In_Dispatch_Trigger p th.(dispatch_trigger)).
 
-(* begin hide *)
+(*| .. coq:: none |*)
 Lemma Dispatch_Frozen_dec:
   forall p th, { Dispatch_Frozen p th } + { ~ Dispatch_Frozen p th }.
 Proof.
@@ -426,7 +463,7 @@ Proof.
   apply dec_sumbool_not.
   apply Feature_In_Dispatch_Trigger_dec.
 Defined.
-(* end hide *)
+(*| .. coq::  |*)
 
 Definition Frozen (p : port_variable) (th : thread_state_variable) : Prop :=
   match Current_Valid_IO_Time_Spec p th with
@@ -440,254 +477,322 @@ Definition Frozen (p : port_variable) (th : thread_state_variable) : Prop :=
 Definition Frozen_Ports' (th : thread_state_variable): list port_variable :=
   filter_dec port_variable_wf port_variable_wf_dec th.(input_ports).
 
-(** ** Runtime support for threads *)
+(*|
+Runtime support for threads -- Private API
+-------------------------------------------
+|*)
 
-(* begin hide *)
+(*| .. coq:: none |*)
 Section Thread_RTS.
-(* end hide *)
+(*| .. coq::  |*)
 
-(** %\N% A collection of runtime services is provided. A runtime service manipulates the thread state and its port variables. *)
+(*| A collection of runtime services is provided. A runtime service manipulates the thread state and its port variables. *)
 
-(** %\define{advance\_time (Coq)}{advance\_time (Coq)}
-{$advance\_time(th, t)$ increments the clock of the thread state variable:\\
-  $$\infer[advance\_time(th, t)]{th() \rightarrow th (clock \leftarrow clock + t)}{th, t \geq 0}$$
-}
-   %*)
+(*| :coq:`advance_time` increments the clock of the thread state variable. |*)
 
-  Definition advance_time (th : thread_state_variable) (t : AADL_Time) := {|
-      (* Generic part *)
-      dispatch_protocol := th.(dispatch_protocol);
-      period := th.(period);
-      deadline := th.(deadline);
-      priority := th.(priority);
-      dispatch_able := th.(dispatch_able);
-
-      input_ports := th.(input_ports);
-      output_ports := th.(output_ports);
-      dispatch_trigger := th.(dispatch_trigger);
-      current_state := th.(current_state);
-      dispatch_time := th.(dispatch_time);
-
-      (* advance_time *)
-      clock := th.(clock) + t;
-    |}.
-
-(** %\begin{definition}[store\_in (Coq)]
-This private API function stores a value in an outer\_port of an AADL thread.
-  \end{definition} %*)
-
-  Definition store_in (t : thread_state_variable) (name : identifier) (value : bool) := {|
-    (* Generic part *)
-    dispatch_protocol := t.(dispatch_protocol);
-    period := t.(period);
-    deadline := t.(deadline);
-    priority := t.(priority);
-    dispatch_able := t.(dispatch_able);
-
-    clock := t.(clock);
-    output_ports := t.(output_ports);
-    dispatch_trigger := t.(dispatch_trigger);
-    current_state := t.(current_state);
-    dispatch_time := t.(dispatch_time);
-
-    (* store_in *)
-    input_ports := Store t.(input_ports) name (t.(clock), value);
-
-  |}.
-
-  Definition update_thread_state (t : thread_state_variable) :=
-  let is_enabled := Enabled_oracle t in {|
+Definition advance_time (th : thread_state_variable) (t : Time) (n : Time) := {|
   (* Generic part *)
-    dispatch_protocol := t.(dispatch_protocol);
-    period := t.(period);
-    deadline := t.(deadline);
-    priority := t.(priority);
-    dispatch_able := t.(dispatch_able);
+  dispatch_protocol := th.(dispatch_protocol);
+  period := th.(period);
+  deadline := th.(deadline);
+  priority := th.(priority);
+  dispatch_able := th.(dispatch_able);
+  wcet := th.(wcet);
 
-    clock := t.(clock);
-    output_ports := t.(output_ports);
-    dispatch_trigger := t.(dispatch_trigger);
-    input_ports := t.(input_ports);
+  input_ports := th.(input_ports);
+  output_ports := th.(output_ports);
+  dispatch_trigger := th.(dispatch_trigger);
+  current_state := th.(current_state);
+  next_dispatch_time := th.(next_dispatch_time);
 
-    (* update_thread_state *)
-    current_state := if is_enabled then Ready else t.(current_state);
-    dispatch_time := if is_enabled then t.(clock) else t.(dispatch_time);
-  |}.
+  (* advance_time *)
+  clock := t;
+  delta_cet := n;
+  cet := th.(cet);
+|}.
 
+Definition compute_during (th : thread_state_variable) (t : Time) := {|
+  (* Generic part *)
+  dispatch_protocol := th.(dispatch_protocol);
+  period := th.(period);
+  deadline := th.(deadline);
+  priority := th.(priority);
+  dispatch_able := th.(dispatch_able);
+  wcet := th.(wcet);
 
-(** %\begin{definition}[Await\_Dispatch (Coq)]
+  input_ports := th.(input_ports);
+  output_ports := th.(output_ports);
+  dispatch_trigger := th.(dispatch_trigger);
+  current_state := th.(current_state);
+  next_dispatch_time := th.(next_dispatch_time);
 
-  \end{definition} %*)
+  (* compute_during *)
+  clock := th.(clock) + t;
+  cet := th.(cet) + t;
+  delta_cet := t;
+|}.
 
-  Definition await_dispatch (t : thread_state_variable) := {|
-    (* Generic part *)
-    dispatch_protocol := t.(dispatch_protocol);
-    period := t.(period);
-    deadline := t.(deadline);
-    priority := t.(priority);
-    dispatch_able := t.(dispatch_able);
+(*| :coq:`store_in` stores a value in an outer\_port of an AADL thread. |*)
 
-    clock := t.(clock);
-    output_ports := t.(output_ports);
-    dispatch_trigger := t.(dispatch_trigger);
-    input_ports := t.(input_ports);
+Definition store_in
+  (t : thread_state_variable) (name : identifier) (value : bool) := {|
+  (* Generic part *)
+  dispatch_protocol := t.(dispatch_protocol);
+  period := t.(period);
+  deadline := t.(deadline);
+  priority := t.(priority);
+  dispatch_able := t.(dispatch_able);
+  wcet := t.(wcet);
 
-    (* await_dispatch *)
-    current_state := Idle;
-    dispatch_time := 0;
-  |}.
+  clock := t.(clock);
+  cet := t.(cet);
+  delta_cet := t.(delta_cet);
+  output_ports := t.(output_ports);
+  dispatch_trigger := t.(dispatch_trigger);
+  current_state := t.(current_state);
+  next_dispatch_time := t.(next_dispatch_time);
 
-(** %\begin{definition}[Get\_Count (Coq)]
-    subprogram Get\_Count
-    features
-      Portvariable: requires data access; -- reference to port variable
-      CountValue: out parameter Base\_Types::Integer; -- content count of port variable
-    end Get\_Count;
+  (* store_in *)
+  input_ports := Store t.(input_ports) name (t.(clock), value);
+|}.
 
-  \end{definition} %*)
+(*| XXX |*)
+Definition eval_enabled_thread_state (t : thread_state_variable) :=
+let is_enabled := Enabled_oracle t in {|
+(* Generic part *)
+  dispatch_protocol := t.(dispatch_protocol);
+  period := t.(period);
+  deadline := t.(deadline);
+  priority := t.(priority);
+  dispatch_able := t.(dispatch_able);
+  wcet := t.(wcet);
 
-  Definition get_count (t : thread_state_variable) (name : identifier) :=
-    Get_Count t.(input_ports) name.
+  clock := t.(clock); (* XXX should reset the clock if enabled *)
+  cet := t.(cet);
+  delta_cet := t.(delta_cet);
+  output_ports := t.(output_ports);
+  dispatch_trigger := t.(dispatch_trigger);
+  input_ports := t.(input_ports);
 
-(** %\begin{definition}[Put\_Value (Coq)]
-    subprogram Put\_Value
-    features
-      Portvariable: requires data access; -- reference to port variable
-      DataValue: in parameter; -- value to be stored
-      DataSize: in parameter;  - size in bytes (optional)
-    end Put\_Value;
-  \end{definition} %*)
+  (* eval_enabled_thread_state *)
+  current_state := if is_enabled then Ready else t.(current_state);
+  next_dispatch_time :=
+    if is_enabled then
+      match t.(dispatch_protocol) with
+      | Periodic =>  t.(clock) + t.(period)
+      | Sporadic =>  t.(clock) + t.(period)
+      | _ => t.(clock)
+      end
+    else t.(next_dispatch_time);
+|}.
 
-  Definition put_value (t : thread_state_variable) (name : identifier) (value : bool) := {|
-    (* Generic part *)
-    dispatch_protocol := t.(dispatch_protocol);
-    period := t.(period);
-    deadline := t.(deadline);
-    priority := t.(priority);
-    dispatch_able := t.(dispatch_able);
+Definition set_running (t : thread_state_variable) := {|
+  (* Generic part *)
+  dispatch_protocol := t.(dispatch_protocol);
+  period := t.(period);
+  deadline := t.(deadline);
+  priority := t.(priority);
+  dispatch_able := t.(dispatch_able);
+  wcet := t.(wcet);
 
-    clock := t.(clock);
-    input_ports := t.(input_ports);
-    dispatch_trigger := t.(dispatch_trigger);
-    current_state := t.(current_state);
-    dispatch_time := t.(dispatch_time);
+  clock := t.(clock);
+  cet := t.(cet);
+  delta_cet := t.(delta_cet);
+  output_ports := t.(output_ports);
+  dispatch_trigger := t.(dispatch_trigger);
+  input_ports := t.(input_ports);
+  next_dispatch_time := t.(next_dispatch_time);
 
-    (* put_value *)
-    output_ports := Store t.(output_ports) name (t.(clock), value);
+  (* set_running *)
+  current_state := Running;
+|}.
 
-  |}.
+Definition set_Idle (t : thread_state_variable) := {|
+  (* Generic part *)
+  dispatch_protocol := t.(dispatch_protocol);
+  period := t.(period);
+  deadline := t.(deadline);
+  priority := t.(priority);
+  dispatch_able := t.(dispatch_able);
+  wcet := t.(wcet);
 
-(** %\begin{definition}[Send\_Output (Coq)]
+  clock := t.(clock);
+  delta_cet := t.(delta_cet);
+  output_ports := t.(output_ports);
+  dispatch_trigger := t.(dispatch_trigger);
+  input_ports := t.(input_ports);
+  next_dispatch_time := t.(next_dispatch_time);
 
-  \end{definition} %*)
+  (* set_Idle *)
+  current_state := Idle;
+  cet := 0;
+|}.
 
-  Definition send_output (t : thread_state_variable) (name : identifier) := {|
-    (* Generic part *)
-    dispatch_protocol := t.(dispatch_protocol);
-    period := t.(period);
-    deadline := t.(deadline);
-    priority := t.(priority);
-    dispatch_able := t.(dispatch_able);
+(*|
+Runtime support for threads -- AADL RTS
+---------------------------------------
 
-    clock := t.(clock);
-    input_ports := t.(input_ports);
-    dispatch_trigger := t.(dispatch_trigger);
-    current_state := t.(current_state);
-    dispatch_time := t.(dispatch_time);
+The definition of the RTS relies on the port functions presented in XXX.
+|*)
 
-    (* send_output *)
-    output_ports := Send_Output t.(output_ports) name;
+(*| * :coq:`Await_Dispatch` |*)
 
-  |}.
+Definition await_dispatch (t : thread_state_variable) := {|
+  (* Generic part *)
+  dispatch_protocol := t.(dispatch_protocol);
+  period := t.(period);
+  deadline := t.(deadline);
+  priority := t.(priority);
+  dispatch_able := t.(dispatch_able);
+  wcet := t.(wcet);
 
-(** %\begin{definition}[Get\_Value (Coq)]
-  subprogram Get\_Value
-  features
-    Portvariable: requires data access; -- reference to port variable
-    DataValue: out parameter; -- value being retrieved
-       -- Error code
-      ErrorCode: out parameter <implementation-defined error code>;
-  end Get\_Value;
-  \end{definition} %*)
+  clock := t.(clock);
+  output_ports := t.(output_ports);
+  dispatch_trigger := t.(dispatch_trigger);
+  input_ports := t.(input_ports);
+  next_dispatch_time := t.(next_dispatch_time);
 
-  Definition get_value (t : thread_state_variable) (name : identifier) :=
-    Get_Value t.(input_ports) name.
+  (* await_dispatch *)
+  current_state := Idle;
 
-  (** %\begin{definition}[Next\_Value (Coq)]
-  subprogram Next\_Value
-  features
-    Portvariable: requires data access; -- reference to port variable
-       -- Error code
-      ErrorCode: out parameter <implementation-defined error code>;
-  end Next\_Value;
-  \end{definition} %*)
+  cet := 0;
+  delta_cet := 0;
+|}.
 
-  Definition next_value (t : thread_state_variable) (name : identifier) (value : bool) := {|
-    (* Generic part *)
-    dispatch_protocol := t.(dispatch_protocol);
-    period := t.(period);
-    deadline := t.(deadline);
-    priority := t.(priority);
-    dispatch_able := t.(dispatch_able);
+(*| * :coq:`Get_Count` |*)
 
-    clock := t.(clock);
-    output_ports := t.(output_ports);
-    dispatch_trigger := t.(dispatch_trigger);
-    current_state := t.(current_state);
-    dispatch_time := t.(dispatch_time);
+Definition get_count (t : thread_state_variable) (name : identifier) :=
+  Get_Count t.(input_ports) name.
 
-    (* next_value *)
-    input_ports := Next_Value t.(input_ports) name;
-  |}.
+(*| * :coq:`Put_Value` |*)
 
-  (** %\begin{definition}[Receive\_Input (Coq)]
-  \end{definition} %*)
+Definition put_value
+  (t : thread_state_variable) (name : identifier) (value : bool) := {|
+  (* Generic part *)
+  dispatch_protocol := t.(dispatch_protocol);
+  period := t.(period);
+  deadline := t.(deadline);
+  priority := t.(priority);
+  dispatch_able := t.(dispatch_able);
+  wcet := t.(wcet);
 
-  Definition receive_input (t : thread_state_variable) (name : identifier) := {|
-    (* Generic part *)
-    dispatch_protocol := t.(dispatch_protocol);
-    period := t.(period);
-    deadline := t.(deadline);
-    priority := t.(priority);
-    dispatch_able := t.(dispatch_able);
+  clock := t.(clock);
+  cet := t.(cet);
+  delta_cet := t.(delta_cet);
+  input_ports := t.(input_ports);
+  dispatch_trigger := t.(dispatch_trigger);
+  current_state := t.(current_state);
+  next_dispatch_time := t.(next_dispatch_time);
 
-    clock := t.(clock);
-    output_ports := t.(output_ports);
-    dispatch_trigger := t.(dispatch_trigger);
-    current_state := t.(current_state);
-    dispatch_time := t.(dispatch_time);
+  (* put_value *)
+  output_ports := Store t.(output_ports) name (t.(clock), value);
+|}.
 
-    (* receive_input *)
-    input_ports := Receive_Input t.(input_ports) name;
+(*| * :coq:`Send_Output` |*)
 
-  |}.
+Definition send_output (t : thread_state_variable) (name : identifier) := {|
+  (* Generic part *)
+  dispatch_protocol := t.(dispatch_protocol);
+  period := t.(period);
+  deadline := t.(deadline);
+  priority := t.(priority);
+  dispatch_able := t.(dispatch_able);
+  wcet := t.(wcet);
 
-(* begin hide *)
+  clock := t.(clock);
+  cet := t.(cet);
+  delta_cet := t.(delta_cet);
+  input_ports := t.(input_ports);
+  dispatch_trigger := t.(dispatch_trigger);
+  current_state := t.(current_state);
+  next_dispatch_time := t.(next_dispatch_time);
+
+  (* send_output *)
+  output_ports := Send_Output t.(output_ports) name;
+|}.
+
+(*| * :coq:`Get_Value` |*)
+
+Definition get_value (t : thread_state_variable) (name : identifier) :=
+  Get_Value t.(input_ports) name.
+
+(*| * :coq:`Next_Value` |*)
+
+Definition next_value
+  (t : thread_state_variable) (name : identifier) (value : bool) := {|
+  (* Generic part *)
+  dispatch_protocol := t.(dispatch_protocol);
+  period := t.(period);
+  deadline := t.(deadline);
+  priority := t.(priority);
+  dispatch_able := t.(dispatch_able);
+  wcet := t.(wcet);
+
+  clock := t.(clock);
+  cet := t.(cet);
+  delta_cet := t.(delta_cet);
+  output_ports := t.(output_ports);
+  dispatch_trigger := t.(dispatch_trigger);
+  current_state := t.(current_state);
+  next_dispatch_time := t.(next_dispatch_time);
+
+  (* next_value *)
+  input_ports := Next_Value t.(input_ports) name;
+|}.
+
+(*| * :coq:`Receive_Input` |*)
+
+Definition receive_input (t : thread_state_variable) (name : identifier) := {|
+  (* Generic part *)
+  dispatch_protocol := t.(dispatch_protocol);
+  period := t.(period);
+  deadline := t.(deadline);
+  priority := t.(priority);
+  dispatch_able := t.(dispatch_able);
+  wcet := t.(wcet);
+
+  clock := t.(clock);
+  cet := t.(cet);
+  delta_cet := t.(delta_cet);
+  output_ports := t.(output_ports);
+  dispatch_trigger := t.(dispatch_trigger);
+  current_state := t.(current_state);
+  next_dispatch_time := t.(next_dispatch_time);
+
+  (* receive_input *)
+  input_ports := Receive_Input t.(input_ports) name;
+|}.
+
+(*| .. coq:: none |*)
 End Thread_RTS.
-(* end hide *)
+(*| .. coq::  |*)
 
-(** * Examples *)
+(*|
+Examples
+--------
+|*)
 
-(** ** A Periodic Thread *)
+(*|
+A Periodic Thread
+^^^^^^^^^^^^^^^^^
 
-(** In this example, we first build a periodic AADL [Component], we then map it to a [thread_state_variable] and perform some steps on it. *)
+In this example, we first build a periodic AADL :coq:`Component`, we then map it to a :coq:`thread_state_variable` and perform some steps on it. |*)
 
-Definition Periodic_Dispatch := {|
-  P := Dispatch_Protocol_Name; PV := PV_Enum (Id "Periodic"); |}.
+Example A_Periodic_Thread :=
+    thread: "a_periodic_thread" ->| "pack::a_thread_classifier"
+        features: nil
+        subcomponents: nil
+        connections: nil
+        properties: [
+            property: Priority_Name ==>| PV_Int 42 ;
+            property: Dispatch_Protocol_Name ==>| PV_Enum (Id "Periodic") ;
+            property: Period_Name ==>| PV_IntU 500 (PV_Unit (Id "ms")) ;
+            property: Compute_Execution_Time_Name ==>|
+                PV_IntRange (PV_IntU 0 (PV_Unit (Id "ms")))
+                            (PV_IntU 100 (PV_Unit (Id "ms")))
+        ].
 
-Definition A_Priority_Value := {|
-  P := Priority_Name; PV := PV_Int 42; |}.
-
-Definition A_Period := {|
-  P := Period_Name; PV := PV_IntU 3 (PV_Unit (Id "ms")); |}.
-
-Definition A_Periodic_Thread := Component
-  (Id "a_periodic_thread")
-  (thread)
-  (FQN [Id "pack"] (Id "a_periodic_thread_classifier") None)
-  nil
-  nil
-  [ A_Priority_Value ; Periodic_Dispatch ; A_Period ] nil.
+(*| This component is well-formed |*)
 
 Lemma A_Periodic_Thread_wf : Well_Formed_Component_Instance A_Periodic_Thread.
 Proof.
@@ -703,7 +808,7 @@ Qed.
 
 (** - "activate" the thread *)
 
-Definition A_Periodic_Thread_State := update_thread_state A_Periodic_Thread_State_.
+Definition A_Periodic_Thread_State := eval_enabled_thread_state A_Periodic_Thread_State_.
 
 (** - At t = 0, the periodic thread is enabled *)
 
@@ -714,7 +819,7 @@ Qed.
 
 (** - "do something" *)
 
-Definition A_Periodic_Thread_State' := advance_time A_Periodic_Thread_State 2.
+Definition A_Periodic_Thread_State' := advance_time A_Periodic_Thread_State 2 0.
 Definition A_Periodic_Thread_State'' := await_dispatch A_Periodic_Thread_State'.
 
 (** - At t = 2, the periodic thread is not enabled *)
@@ -724,90 +829,362 @@ Proof.
   trivial.
 Qed.
 
-(** ** A Sporadic Thread *)
+(*| Let us turn this thread into a P-DEVS. |*)
 
-(** In this example, we consider a sporadic thread with one input event port. *)
+(*| :coq:`X_thread` is the set of incoming messages the P-DEVS reacts to.  |*)
 
-Definition Sporadic_Dispatch  := {|
-  P := Dispatch_Protocol_Name; PV := PV_Enum (Id "Sporadic"); |}.
+Inductive X_thread : Set :=
+| thread_step
+| eval_enabled  (clock: Time)
+| run_thread (clock : Time) (duration : Time).
 
-Definition An_Input_Feature :=
-  Feature (Id "a_feature") inF eventPort nil_component nil.
+Definition Y_thread : Type := X_thread.
 
-Definition A_Sporadic_Thread := Component
-  (Id "a_sporadic_thread")
-  (thread)
-  (FQN [Id "pack"] (Id "a_sporadic_thread_classifier") None)
-  [ An_Input_Feature ]
-  nil
-  [A_Priority_Value ; Sporadic_Dispatch ; A_Period ]
-  nil.
+Definition Synchronization_Message_Type_thread :=
+    Synchronization_Message_Type X_thread Y_thread.
 
-(** We can continue and build a corresponding thread state variable, add an event, avance time and check whether the thread is enabled. *)
+(*| :coq:`S_thread` is the state variable of the P-DEVS. It is the cross-product of a label denoting the state and the actual state varoable. XXX thread_state_variable also has the Ready/Idle/Run state, is this redundant ?|*)
 
-Definition A_Sporadic_Thread_State_ := mk_thread_state_variable (A_Sporadic_Thread).
+Inductive S_thread_labels : Set :=
+    | performing_thread_activation
+    | suspended_awaiting_dispatch
+    | performing_thread_computation .
 
-Lemma A_Sporadic_Thread_State_valid : thread_state_variable_wf A_Sporadic_Thread_State_.
-Proof.
-  prove_thread_state_variable_wf.
-Qed.
+Record S_thread := {
+  thread_l : S_thread_labels ;
+  thread_st : thread_state_variable ;
+  thread_ce : Compute_Entry_Point;
+  }.
 
-Definition A_Sporadic_Thread_State := update_thread_state A_Sporadic_Thread_State_.
+Definition Update_S_thread
+  (s : S_thread)
+  (label : S_thread_labels)
+  (tsv : thread_state_variable)
+:=
+ {| thread_l := label ; thread_st := tsv; thread_ce := s.(thread_ce) |} .
 
-(** - Initially, the sporadic thread is not enabled *)
+Definition Q_thread : Type := Q S_thread.
 
-Lemma Sporadic_tO_not_enabled : Enabled_oracle (A_Sporadic_Thread_State) = false.
-Proof.
-  trivial.
-Qed.
+(* XXX better definition? *)
+Definition Q_init_thread
+  (tsv : thread_state_variable)
+  (tce : Compute_Entry_Point)
+  : Q_thread :=
+  {| st := {| thread_l := performing_thread_activation ;
+              thread_st := tsv;
+              thread_ce := tce ;
+              |} ;
+    e := Zero |}.
 
-(** - Inject two events. Because of the DropOldest policy used, with a queue size of 1, we loose the first event *)
+Definition Update_Q
+  (q : Q_thread)
+  (label : S_thread_labels)
+  (tsv : thread_state_variable)
+:=
+  {| st := Update_S_thread q.(st) label tsv ; e := q.(e) |}.
 
-Definition A_Sporadic_Thread_State' :=
-  store_in A_Sporadic_Thread_State (Id "a_feature") false.
-Definition A_Sporadic_Thread_State'' :=
-  store_in A_Sporadic_Thread_State' (Id "a_feature") true.
+(*| :coq:`δint_thread` updates the internal state of the thread
 
-(** - The thread is not enabled yet *)
+- (1) if the thread is Idle, we evaluate its enable function using eval_enabled_thread_state. If the thread is Readym we enter the performing thread conputation
 
-Lemma Sporatic_tO_not_enabled' : A_Sporadic_Thread_State''.(current_state) = Idle.
-Proof.
-  trivial.
-Qed.
+- (2) if the thread is Running, and if its compute execution time is equal to its WCET, the thread becomes suspended (external AADL state) and Idle .
 
-(** - We advance time *)
-Definition th_ := advance_time A_Sporadic_Thread_State'' 4.
-Definition th := update_thread_state th_.
+- Otherwise, we keep the existing state
 
-(** - The thread is enabled, and we can check frozen port *)
+|*)
 
-Lemma Sporadic_t42_enabled : th.(current_state) = Ready.
-Proof.
-  trivial.
-Qed.
+Definition δint_thread (s : S_thread) : S_thread :=
+  match s.(thread_st).(current_state) with
 
-Lemma ETF: Get_Port_Variable_Name (Get_Elected_Triggering_Feature (th)) = Id "a_feature".
-Proof.
-  trivial.
-Qed.
+    | Not_Activated  => s
 
-(* - At this stage, we have not called receive_input, no event available *)
+    | Idle => (* (1) *)
+      let state' := eval_enabled_thread_state s.(thread_st) in
+        match state'.(current_state) with
+        | Ready => Update_S_thread s performing_thread_computation state'
 
-Lemma get_count_1 : get_count th (Id "a_feature") = 0%nat.
-Proof.
-  trivial.
-Qed.
+        | _ =>  s
+        end
 
-(* - Calling receive input *)
+    | Running => (* (2) *)
+    (* XXX must split compute_entrypoint into parts: await/fetch/execute/write
+all atomic except execute
 
-Definition th_rec := receive_input th (Id "a_feature").
+    *)
+      let state := s.(thread_ce) s.(thread_st) in
 
-Lemma get_count_2 : get_count th_rec (Id "a_feature") = 1%nat.
-Proof.
-  trivial.
-Qed.
+      if state.(wcet) <=? state.(cet) then
+        {| thread_l := suspended_awaiting_dispatch ;
+           thread_st := set_Idle state ;
+           thread_ce := s.(thread_ce) |}
 
-Lemma get_value_1 : get_value th_rec (Id "a_feature") = (0,true).
-Proof.
-  trivial.
-Qed.
+      else
+        {| thread_l := performing_thread_computation;
+           thread_st := state;
+           thread_ce := s.(thread_ce) |}
+
+    | Ready  => s
+  end.
+
+(*| :coq:`δext_thread` take into account incoming messages to update
+the thread state. |*)
+Definition δext_thread (q : Q_thread) (x : list X_thread) : S_thread :=
+  match q.(st).(thread_l), hd_error x with
+
+    | performing_thread_activation, Some thread_step =>
+    let state' := await_dispatch q.(st).(thread_st) in
+      {| thread_l  := suspended_awaiting_dispatch ;
+         thread_st := state' ;
+         thread_ce := q.(st).(thread_ce) |}
+
+    | suspended_awaiting_dispatch, Some (eval_enabled c) =>
+      let state' := advance_time q.(st).(thread_st) c 0 in
+        {| thread_l  := q.(st).(thread_l) ;
+          thread_st := state' ;
+          thread_ce := q.(st).(thread_ce) |}
+
+    | performing_thread_computation, Some (run_thread c n) =>
+      let state := set_running q.(st).(thread_st) in
+      let state' := advance_time state c n in
+        {| thread_l := performing_thread_computation ;
+          thread_st := state' ;
+          thread_ce := q.(st).(thread_ce) |}
+
+    | _, _ => q.(st)
+
+end.
+
+Definition δcon_thread  := Build_Default_δcon δint_thread δext_thread.
+
+Definition Y_output_thread : Type := Y_output Y_thread.
+
+Definition λ_thread (s : S_thread) : list Y_output_thread :=
+  match s with
+    | _ => [ no_output Y_thread ]
+  end.
+
+Definition ta_thread (s : S_thread) : Time :=
+  match s.(thread_l) with
+    | performing_thread_activation => Zero
+    | suspended_awaiting_dispatch =>
+        s.(thread_st).(next_dispatch_time) + s.(thread_st).(delta_cet)
+        - s.(thread_st).(clock)
+    | performing_thread_computation => s.(thread_st).(delta_cet)
+  end.
+
+Definition thread_DEVS_type : Type :=
+    DEVS_Atomic_Model S_thread X_thread Y_thread.
+
+Definition Periodic_Compute_Entry_Point : Compute_Entry_Point :=
+  fun x : thread_state_variable =>
+    compute_during x x.(delta_cet).
+
+Definition thread_DEVS
+    (t : component)
+    (ce : Compute_Entry_Point)
+    : thread_DEVS_type := {|
+    devs_atomic_id := t->id ;
+    Q_init := Q_init_thread (mk_thread_state_variable t) ce;
+
+    ta := ta_thread;
+    δint := δint_thread;
+    λ  := λ_thread;
+    δext := δext_thread;
+    δcon := δcon_thread;
+|}.
+
+Definition thread_DEVS_Simulator_Type : Type :=
+    DEVS_Simulator S_thread X_thread Y_thread.
+
+Definition thread_Initial (t : component) := Instantiate_DEVS_Simulator
+    (Id "thread") (thread_DEVS t Periodic_Compute_Entry_Point).
+
+(* Translate DEVS to a LTS *)
+
+Definition A_Periodic_initial := thread_Initial A_Periodic_Thread.
+
+Definition thread_LTS := LTS_Of_DEVS (A_Periodic_initial).
+
+Example thread_LTS_0 := Init thread_LTS.
+
+(*| * Step#0: we confirm the correct initialization of a thread |*)
+
+Lemma thread_LTS_0_OK :
+    Print_DEVS_Simulator thread_LTS_0 =
+    dbg Zero Zero
+    {|
+      thread_l := performing_thread_activation;
+      thread_st :=
+        {|
+          dispatch_protocol := Periodic;
+          period := 500;
+          deadline := 0%Z;
+          priority := 42;
+          dispatch_able := true;
+          wcet := 100;
+          clock := 0;
+          cet := 0;
+          delta_cet := 0;
+          current_state := Not_Activated;
+          next_dispatch_time := 0;
+          input_ports := [];
+          output_ports := [];
+          dispatch_trigger := []
+        |};
+        thread_ce := Periodic_Compute_Entry_Point;
+    |} [].
+Proof. trivial. Qed.
+
+(*| * Step#1: We perform a :coq:`thread_step` to activate the thread. Because of the activation time allows the thread to be dispatched, the thread directly enters the :coq:`performing_thread_computation` state. This is expected because of the confluence function that executes first the external transition, then the internal one. |*)
+
+Example thread_LTS_1 :=
+  step_lts thread_LTS_0
+    (xs Y_thread Parent Parent Zero [ thread_step ]).
+
+Lemma thread_LTS_1_OK :
+    Print_DEVS_Simulator thread_LTS_1 =
+    dbg Zero Zero
+    {|
+      thread_l := performing_thread_computation;
+      thread_st :=
+        {|
+          dispatch_protocol := Periodic;
+          period := 500;
+          deadline := 0%Z;
+          priority := 42;
+          dispatch_able := true;
+          wcet := 100;
+          clock := 0;
+          cet := 0;
+          delta_cet := 0;
+          current_state := Ready;
+          next_dispatch_time := 500;
+          input_ports := [];
+          output_ports := [];
+          dispatch_trigger := []
+        |};
+        thread_ce := Periodic_Compute_Entry_Point;
+    |} [].
+Proof. trivial. Qed.
+
+(*| * Step#2: we "run" the thread for 50 ms |*)
+
+Example thread_LTS_2 :=
+    step_lts thread_LTS_1
+    (xs Y_thread Parent Parent Zero [ run_thread 0 50 ]).
+
+Lemma thread_LTS_2_OK :
+    Print_DEVS_Simulator thread_LTS_2 =
+    dbg 0 50
+    {|
+      thread_l := performing_thread_computation;
+      thread_st :=
+        {|
+          dispatch_protocol := Periodic;
+          period := 500;
+          deadline := 0%Z;
+          priority := 42;
+          dispatch_able := true;
+          wcet := 100;
+          clock := 50;
+          cet := 50;
+          delta_cet := 50;
+          current_state := Running;
+          next_dispatch_time := 500;
+          input_ports := [];
+          output_ports := [];
+          dispatch_trigger := []
+        |};
+        thread_ce := Periodic_Compute_Entry_Point;
+    |} [].
+Proof. trivial. Qed.
+
+(*| * Step#3: we "run" the thread for another 50 ms to see it being completed and go back to :coq:`suspended_awaiting_dispatch` state. |*)
+
+Example thread_LTS_3 :=
+    step_lts thread_LTS_2 (xs Y_thread Parent Parent 50%nat [ run_thread 50 50%nat ]).
+
+Lemma thread_LTS_3_OK :
+    Print_DEVS_Simulator thread_LTS_3 =
+    dbg 50%nat 500%nat
+    {|
+      thread_l := suspended_awaiting_dispatch;
+      thread_st :=
+        {|
+          dispatch_protocol := Periodic;
+          period := 500;
+          deadline := 0%Z;
+          priority := 42;
+          dispatch_able := true;
+          wcet := 100;
+          clock := 100; (* XXX *)
+          cet := 0;
+          delta_cet := 50;
+          current_state := Idle;
+          next_dispatch_time := 500;
+          input_ports := [];
+          output_ports := [];
+          dispatch_trigger := []
+        |};
+        thread_ce := Periodic_Compute_Entry_Point;
+    |} [].
+Proof. trivial. Qed.
+
+Example thread_LTS_4 :=
+    step_lts thread_LTS_3
+    (xs Y_thread Parent Parent 500 [ eval_enabled 500 ]).
+
+Lemma thread_LTS_4_OK :
+    Print_DEVS_Simulator thread_LTS_4 =
+    dbg 500 500
+    {|
+      thread_l := performing_thread_computation;
+      thread_st :=
+             {|
+               dispatch_protocol := Periodic;
+               period := 500;
+               deadline := 0%Z;
+               priority := 42;
+               dispatch_able := true;
+               wcet := 100;
+               clock := 500;
+               cet := 0;
+               delta_cet := 0;
+               current_state := Ready;
+               next_dispatch_time := 1000;
+               input_ports := [];
+               output_ports := [];
+               dispatch_trigger := []
+             |};
+        thread_ce := Periodic_Compute_Entry_Point;
+    |} [].
+Proof. trivial. Qed.
+
+Example thread_LTS_5 :=
+    step_lts thread_LTS_4 (xs Y_thread Parent Parent 500 [ run_thread 500 100%nat ]).
+
+Lemma thread_LTS_5_OK :
+    Print_DEVS_Simulator thread_LTS_5 =
+    dbg 500 1000
+         {|
+           thread_l := suspended_awaiting_dispatch;
+           thread_st :=
+             {|
+               dispatch_protocol := Periodic;
+               period := 500;
+               deadline := 0%Z;
+               priority := 42;
+               dispatch_able := true;
+               wcet := 100;
+               clock := 600;
+               cet := 0;
+               delta_cet := 100;
+               current_state := Idle;
+               next_dispatch_time := 1000;
+               input_ports := [];
+               output_ports := [];
+               dispatch_trigger := []
+             |};
+          thread_ce := Periodic_Compute_Entry_Point;
+          |} [].
+Proof. trivial. Qed.
